lecture_12.v
@@ -1,0 +1,189 @@
+(* import string *)
+From Coq Require Import Bool.Bool.
+From Coq Require Import Init.Nat.
+From Coq Require Import Arith.Arith.
+From Coq Require Import Arith.EqNat.
+Import Nat.
+From Coq Require Import Lia.
+From Coq Require Import Lists.List.
+From Coq Require Import Strings.String.
+Import ListNotations.
+Open Scope string_scope.
+
+
+
+(* define map *)
+Definition total_map (A : Type) := string -> A.
+Definition t_empty {A:Type} (v : A) : total_map A := (fun _ => v).
+Definition t_update {A:Type} (m : total_map A) (x : string) (v : A) :=
+    fun x' => if string_dec x x' then v else m x'.
+
+
+Notation "x '!->' v" := (t_update (t_empty v) x v) (at level 100).
+Notation "x '!->' v ';' m" := (t_update m x v)
+                              (at level 100, v at next level, right associativity).
+
+(** ** States *)
+
+(** Since we'll want to look variables up to find out their current
+    values, we'll reuse maps from the [Maps] chapter, and
+    [string]s will be used to represent variables in Imp.
+
+    A _machine state_ (or just _state_) represents the current values
+    of _all_ variables at some point in the execution of a program. *)
+
+(** For simplicity, we assume that the state is defined for
+    _all_ variables, even though any given program is only going to
+    mention a finite number of them.  The state captures all of the
+    information stored in memory.  For Imp programs, because each
+    variable stores a natural number, we can represent the state as a
+    mapping from strings to [nat], and will use [0] as default value
+    in the store. For more complex programming languages, the state
+    might have more structure. *)
+
+Definition state := total_map nat.
+(* import maps *)
+Inductive aexp : Type :=
+  | ANum (n : nat)
+  | AId (x : string)              (* <--- NEW *)
+  | APlus (a1 a2 : aexp)
+  | AMinus (a1 a2 : aexp)
+  | AMult (a1 a2 : aexp).
+
+(** Defining a few variable names as notational shorthands will make
+    examples easier to read: *)
+
+Definition W : string := "W".
+Definition X : string := "X".
+Definition Y : string := "Y".
+Definition Z : string := "Z".
+
+(** (This convention for naming program variables ([X], [Y],
+    [Z]) clashes a bit with our earlier use of uppercase letters for
+    types.  Since we're not using polymorphism heavily in the chapters
+    developed to Imp, this overloading should not cause confusion.) *)
+
+(** The definition of [bexp]s is unchanged (except that it now refers
+    to the new [aexp]s): *)
+
+Inductive bexp : Type :=
+  | BTrue
+  | BFalse
+  | BEq (a1 a2 : aexp)
+  | BLe (a1 a2 : aexp)
+  | BNot (b : bexp)
+  | BAnd (b1 b2 : bexp).
+
+(* ================================================================= *)
+(** ** Notations *)
+
+(** To make Imp programs easier to read and write, we introduce some
+    notations and implicit coercions.  You do not need to understand
+    exactly what these declarations do.  Briefly, though:
+       - The [Coercion] declaration stipulates that a function (or
+         constructor) can be implicitly used by the type system to
+         coerce a value of the input type to a value of the output
+         type.  For instance, the coercion declaration for [AId]
+         allows us to use plain strings when an [aexp] is expected;
+         the string will implicitly be wrapped with [AId].
+       - [Declare Custom Entry com] tells Coq to create a new
+         "custom grammar" for parsing Imp expressions and
+         programs. The first notation declaration after this tells Coq
+         that anything between [<{] and [}>] should be parsed using
+         the Imp grammar. Again, it is not necessary to understand the
+         details, but it is important to recognize that we are
+         defining _new_ interpretations for some familiar operators
+         like [+], [-], [*], [=], [<=], etc., when they occur between
+         [<{] and [}>]. *)
+
+Coercion AId : string >-> aexp.
+Coercion ANum : nat >-> aexp.
+
+Declare Custom Entry com.
+Declare Scope com_scope.
+Notation "<{ e }>" := e (at level 0, e custom com at level 99) : com_scope.
+Notation "( x )" := x (in custom com, x at level 99) : com_scope.
+Notation "x" := x (in custom com at level 0, x constr at level 0) : com_scope.
+Notation "f x .. y" := (.. (f x) .. y)
+                  (in custom com at level 0, only parsing,
+                  f constr at level 0, x constr at level 9,
+                  y constr at level 9) : com_scope.
+Notation "x + y" := (APlus x y) (in custom com at level 50, left associativity).
+Notation "x - y" := (AMinus x y) (in custom com at level 50, left associativity).
+Notation "x * y" := (AMult x y) (in custom com at level 40, left associativity).
+Notation "'true'"  := true (at level 1).
+Notation "'true'"  := BTrue (in custom com at level 0).
+Notation "'false'"  := false (at level 1).
+Notation "'false'"  := BFalse (in custom com at level 0).
+Notation "x <= y" := (BLe x y) (in custom com at level 70, no associativity).
+Notation "x = y"  := (BEq x y) (in custom com at level 70, no associativity).
+Notation "x && y" := (BAnd x y) (in custom com at level 80, left associativity).
+Notation "'~' b"  := (BNot b) (in custom com at level 75, right associativity).
+
+Open Scope com_scope.
+Definition example_aexp : aexp := <{ 3 + (X * 2) }>.
+Definition example_bexp : bexp := <{ true && ~(X <= 4) }>.
+(** One downside of these and notation tricks -- coercions in
+    particular -- is that they can make it a little harder for humans
+    to calculate the types of expressions.  If you ever find yourself
+    confused, try doing [Set Printing Coercions] to see exactly what
+    is going on. *)
+
+Print example_bexp.
+(* ===> example_bexp = <{(true && ~ (X <= 4))}> *)
+
+Set Printing Coercions.
+Print example_bexp.
+(* ===> example_bexp = <{(true && ~ (AId X <= ANum 4))}> *)
+
+Unset Printing Coercions.
+
+(* ================================================================= *)
+(** ** Evaluation *)
+
+(** The arith and boolean evaluators are extended to handle
+    variables in the obvious way, taking a state as an extra
+    argument: *)
+
+Fixpoint aeval (st : state) (a : aexp) : nat :=
+  match a with
+  | ANum n => n
+  | AId x => st x                                (* <--- NEW *)
+  | <{a1 + a2}> => (aeval st a1) + (aeval st a2)
+  | <{a1 - a2}> => (aeval st a1) - (aeval st a2)
+  | <{a1 * a2}> => (aeval st a1) * (aeval st a2)
+  end.
+(* dunno why this doesnt work *)
+Fixpoint beval (st : state) (b : bexp) : bool :=
+  match b with
+  | <{true}>      => true
+  | <{false}>     => false
+  | <{a1 = a2}>   => (aeval st a1) =? (aeval st a2)
+  | <{a1 <= a2}>  => (aeval st a1) <=? (aeval st a2)
+  | <{~ b1}>      => negb (beval st b1)
+  | <{b1 && b2}>  => andb (beval st b1) (beval st b2)
+  end.
+
+(** We specialize our notation for total maps to the specific case of
+    states, i.e. using [(_ !-> 0)] as empty state. *)
+
+Definition empty_st := (_ !-> 0).
+
+(** Now we can add a notation for a "singleton state" with just one
+    variable bound to a value. *)
+Notation "x '!->' v" := (x !-> v ; empty_st) (at level 100).
+
+Example aexp1 :
+    aeval (X !-> 5) <{ 3 + (X * 2) }>
+  = 13.
+Proof. reflexivity. Qed.
+
+Example aexp2 :
+    aeval (X !-> 5 ; Y !-> 4) <{ Z + (X * Y) }>
+  = 20.
+Proof. reflexivity. Qed.
+
+Example bexp1 :
+    beval (X !-> 5) <{ true && ~(X <= 4) }>
+  = true.
+Proof. reflexivity. Qed.
